port WP_revisited in progress

examples/WP_revisited/blocking_semantics5/blocking_semantics5_TestSemantics_If42_1.v
@@ -2,6 +2,7 @@
 (* Beware! Only edit allowed sections below    *)
 Require Import BuiltIn.
 Require BuiltIn.
+Require HighOrd.
 Require bool.Bool.
 Require int.Int.
 Require map.Map.
@@ -80,7 +81,7 @@ Existing Instance stmt_WhyType.
 Axiom decide_is_skip : forall (s:stmt), (s = Sskip) \/ ~ (s = Sskip).
 
 (* Why3 assumption *)
-Definition env := (map.Map.map mident value).
+Definition env := (mident -> value).
 
 (* Why3 assumption *)
 Definition stack := (list (ident* value)%type).
@@ -117,19 +118,19 @@ Axiom eval_bin_def : forall (x:value) (op:operator) (y:value), match (x,
   end.
 
 (* Why3 assumption *)
-Fixpoint eval_term (sigma:(map.Map.map mident value)) (pi:(list (ident*
-  value)%type)) (t:term) {struct t}: value :=
+Fixpoint eval_term (sigma:(mident -> value)) (pi:(list (ident* value)%type))
+  (t:term) {struct t}: value :=
   match t with
   | (Tvalue v) => v
   | (Tvar id) => (get_stack id pi)
-  | (Tderef id) => (map.Map.get sigma id)
+  | (Tderef id) => (sigma id)
   | (Tbin t1 op t2) => (eval_bin (eval_term sigma pi t1) op (eval_term sigma
       pi t2))
   end.
 
 (* Why3 assumption *)
-Fixpoint eval_fmla (sigma:(map.Map.map mident value)) (pi:(list (ident*
-  value)%type)) (f:fmla) {struct f}: Prop :=
+Fixpoint eval_fmla (sigma:(mident -> value)) (pi:(list (ident* value)%type))
+  (f:fmla) {struct f}: Prop :=
   match f with
   | (Fterm t) => ((eval_term sigma pi t) = (Vbool true))
   | (Fand f1 f2) => (eval_fmla sigma pi f1) /\ (eval_fmla sigma pi f2)
@@ -146,70 +147,62 @@ Fixpoint eval_fmla (sigma:(map.Map.map mident value)) (pi:(list (ident*
   end.
 
 (* Why3 assumption *)
-Definition valid_fmla (p:fmla): Prop := forall (sigma:(map.Map.map mident
-  value)) (pi:(list (ident* value)%type)), (eval_fmla sigma pi p).
+Definition valid_fmla (p:fmla): Prop := forall (sigma:(mident -> value))
+  (pi:(list (ident* value)%type)), (eval_fmla sigma pi p).
 
 (* Why3 assumption *)
-Inductive one_step: (map.Map.map mident value) -> (list (ident*
-  value)%type) -> stmt -> (map.Map.map mident value) -> (list (ident*
-  value)%type) -> stmt -> Prop :=
-  | one_step_assign : forall (sigma:(map.Map.map mident value))
-      (sigma':(map.Map.map mident value)) (pi:(list (ident* value)%type))
-      (x:mident) (t:term), (sigma' = (map.Map.set sigma x (eval_term sigma pi
-      t))) -> (one_step sigma pi (Sassign x t) sigma' pi Sskip)
-  | one_step_seq_noskip : forall (sigma:(map.Map.map mident value))
-      (sigma':(map.Map.map mident value)) (pi:(list (ident* value)%type))
-      (pi':(list (ident* value)%type)) (s1:stmt) (s1':stmt) (s2:stmt),
-      (one_step sigma pi s1 sigma' pi' s1') -> (one_step sigma pi (Sseq s1
-      s2) sigma' pi' (Sseq s1' s2))
-  | one_step_seq_skip : forall (sigma:(map.Map.map mident value))
-      (pi:(list (ident* value)%type)) (s:stmt), (one_step sigma pi
-      (Sseq Sskip s) sigma pi s)
-  | one_step_if_true : forall (sigma:(map.Map.map mident value))
-      (pi:(list (ident* value)%type)) (t:term) (s1:stmt) (s2:stmt),
-      ((eval_term sigma pi t) = (Vbool true)) -> (one_step sigma pi (Sif t s1
-      s2) sigma pi s1)
-  | one_step_if_false : forall (sigma:(map.Map.map mident value))
-      (pi:(list (ident* value)%type)) (t:term) (s1:stmt) (s2:stmt),
-      ((eval_term sigma pi t) = (Vbool false)) -> (one_step sigma pi (Sif t
-      s1 s2) sigma pi s2)
-  | one_step_assert : forall (sigma:(map.Map.map mident value))
-      (pi:(list (ident* value)%type)) (f:fmla), (eval_fmla sigma pi f) ->
-      (one_step sigma pi (Sassert f) sigma pi Sskip)
-  | one_step_while_true : forall (sigma:(map.Map.map mident value))
-      (pi:(list (ident* value)%type)) (cond:term) (inv:fmla) (body:stmt),
-      ((eval_fmla sigma pi inv) /\ ((eval_term sigma pi
-      cond) = (Vbool true))) -> (one_step sigma pi (Swhile cond inv body)
-      sigma pi (Sseq body (Swhile cond inv body)))
-  | one_step_while_false : forall (sigma:(map.Map.map mident value))
-      (pi:(list (ident* value)%type)) (cond:term) (inv:fmla) (body:stmt),
-      ((eval_fmla sigma pi inv) /\ ((eval_term sigma pi
-      cond) = (Vbool false))) -> (one_step sigma pi (Swhile cond inv body)
-      sigma pi Sskip).
+Inductive one_step: (mident -> value) -> (list (ident* value)%type) ->
+  stmt -> (mident -> value) -> (list (ident* value)%type) -> stmt -> Prop :=
+  | one_step_assign : forall (sigma:(mident -> value)) (sigma':(mident ->
+      value)) (pi:(list (ident* value)%type)) (x:mident) (t:term),
+      (sigma' = (map.Map.set sigma x (eval_term sigma pi t))) -> (one_step
+      sigma pi (Sassign x t) sigma' pi Sskip)
+  | one_step_seq_noskip : forall (sigma:(mident -> value)) (sigma':(mident ->
+      value)) (pi:(list (ident* value)%type)) (pi':(list (ident*
+      value)%type)) (s1:stmt) (s1':stmt) (s2:stmt), (one_step sigma pi s1
+      sigma' pi' s1') -> (one_step sigma pi (Sseq s1 s2) sigma' pi' (Sseq s1'
+      s2))
+  | one_step_seq_skip : forall (sigma:(mident -> value)) (pi:(list (ident*
+      value)%type)) (s:stmt), (one_step sigma pi (Sseq Sskip s) sigma pi s)
+  | one_step_if_true : forall (sigma:(mident -> value)) (pi:(list (ident*
+      value)%type)) (t:term) (s1:stmt) (s2:stmt), ((eval_term sigma pi
+      t) = (Vbool true)) -> (one_step sigma pi (Sif t s1 s2) sigma pi s1)
+  | one_step_if_false : forall (sigma:(mident -> value)) (pi:(list (ident*
+      value)%type)) (t:term) (s1:stmt) (s2:stmt), ((eval_term sigma pi
+      t) = (Vbool false)) -> (one_step sigma pi (Sif t s1 s2) sigma pi s2)
+  | one_step_assert : forall (sigma:(mident -> value)) (pi:(list (ident*
+      value)%type)) (f:fmla), (eval_fmla sigma pi f) -> (one_step sigma pi
+      (Sassert f) sigma pi Sskip)
+  | one_step_while_true : forall (sigma:(mident -> value)) (pi:(list (ident*
+      value)%type)) (cond:term) (inv:fmla) (body:stmt), ((eval_fmla sigma pi
+      inv) /\ ((eval_term sigma pi cond) = (Vbool true))) -> (one_step sigma
+      pi (Swhile cond inv body) sigma pi (Sseq body (Swhile cond inv body)))
+  | one_step_while_false : forall (sigma:(mident -> value)) (pi:(list (ident*
+      value)%type)) (cond:term) (inv:fmla) (body:stmt), ((eval_fmla sigma pi
+      inv) /\ ((eval_term sigma pi cond) = (Vbool false))) -> (one_step sigma
+      pi (Swhile cond inv body) sigma pi Sskip).
 
 (* Why3 assumption *)
-Inductive many_steps: (map.Map.map mident value) -> (list (ident*
-  value)%type) -> stmt -> (map.Map.map mident value) -> (list (ident*
-  value)%type) -> stmt -> Z -> Prop :=
-  | many_steps_refl : forall (sigma:(map.Map.map mident value))
-      (pi:(list (ident* value)%type)) (s:stmt), (many_steps sigma pi s sigma
-      pi s 0%Z)
-  | many_steps_trans : forall (sigma1:(map.Map.map mident value))
-      (sigma2:(map.Map.map mident value)) (sigma3:(map.Map.map mident value))
-      (pi1:(list (ident* value)%type)) (pi2:(list (ident* value)%type))
-      (pi3:(list (ident* value)%type)) (s1:stmt) (s2:stmt) (s3:stmt) (n:Z),
-      (one_step sigma1 pi1 s1 sigma2 pi2 s2) -> ((many_steps sigma2 pi2 s2
-      sigma3 pi3 s3 n) -> (many_steps sigma1 pi1 s1 sigma3 pi3 s3
-      (n + 1%Z)%Z)).
+Inductive many_steps: (mident -> value) -> (list (ident* value)%type) ->
+  stmt -> (mident -> value) -> (list (ident* value)%type) -> stmt -> Z ->
+  Prop :=
+  | many_steps_refl : forall (sigma:(mident -> value)) (pi:(list (ident*
+      value)%type)) (s:stmt), (many_steps sigma pi s sigma pi s 0%Z)
+  | many_steps_trans : forall (sigma1:(mident -> value)) (sigma2:(mident ->
+      value)) (sigma3:(mident -> value)) (pi1:(list (ident* value)%type))
+      (pi2:(list (ident* value)%type)) (pi3:(list (ident* value)%type))
+      (s1:stmt) (s2:stmt) (s3:stmt) (n:Z), (one_step sigma1 pi1 s1 sigma2 pi2
+      s2) -> ((many_steps sigma2 pi2 s2 sigma3 pi3 s3 n) -> (many_steps
+      sigma1 pi1 s1 sigma3 pi3 s3 (n + 1%Z)%Z)).
 
-Axiom steps_non_neg : forall (sigma1:(map.Map.map mident value))
-  (sigma2:(map.Map.map mident value)) (pi1:(list (ident* value)%type))
-  (pi2:(list (ident* value)%type)) (s1:stmt) (s2:stmt) (n:Z), (many_steps
-  sigma1 pi1 s1 sigma2 pi2 s2 n) -> (0%Z <= n)%Z.
+Axiom steps_non_neg : forall (sigma1:(mident -> value)) (sigma2:(mident ->
+  value)) (pi1:(list (ident* value)%type)) (pi2:(list (ident* value)%type))
+  (s1:stmt) (s2:stmt) (n:Z), (many_steps sigma1 pi1 s1 sigma2 pi2 s2 n) ->
+  (0%Z <= n)%Z.
 
 (* Why3 assumption *)
-Definition reductible (sigma:(map.Map.map mident value)) (pi:(list (ident*
-  value)%type)) (s:stmt): Prop := exists sigma':(map.Map.map mident value),
+Definition reductible (sigma:(mident -> value)) (pi:(list (ident*
+  value)%type)) (s:stmt): Prop := exists sigma':(mident -> value),
   exists pi':(list (ident* value)%type), exists s':stmt, (one_step sigma pi s
   sigma' pi' s').
 
@@ -221,15 +214,13 @@ Require Import Why3.
 Ltac ae := why3 "Alt-Ergo,0.99.1," timelimit 3; admit.
 
 (* Why3 goal *)
-Theorem If42 : forall (sigma1:(map.Map.map mident value))
-  (sigma2:(map.Map.map mident value)) (pi1:(list (ident* value)%type))
-  (pi2:(list (ident* value)%type)) (s:stmt), (one_step
-  (map.Const.const (Vint 0%Z): (map.Map.map mident value))
+Theorem If42 : forall (sigma1:(mident -> value)) (sigma2:(mident -> value))
+  (pi1:(list (ident* value)%type)) (pi2:(list (ident* value)%type)) (s:stmt),
+  (one_step (map.Const.const (Vint 0%Z): (mident -> value))
   (Init.Datatypes.cons (x, (Vint 42%Z)) Init.Datatypes.nil)
   (Sif (Tbin (Tderef y) Ole (Tvalue (Vint 10%Z))) (Sassign y
   (Tvalue (Vint 13%Z))) (Sassign y (Tvalue (Vint 42%Z)))) sigma1 pi1 s) ->
-  ((one_step sigma1 pi1 s sigma2 pi2 Sskip) -> ((map.Map.get sigma2
-  y) = (Vint 13%Z))).
+  ((one_step sigma1 pi1 s sigma2 pi2 Sskip) -> ((sigma2 y) = (Vint 13%Z))).
 (* Why3 intros sigma1 sigma2 pi1 pi2 s h1 h2. *)
 intros sigma1 sigma2 pi1 pi2 s h1 h2.
 inversion h1; subst; clear h1.
