examples/WP_revisited/blocking_semantics5/blocking_semantics5_TypingAndSemantics_eval_type_term_1.v
@@ -2,6 +2,7 @@
 (* Beware! Only edit allowed sections below    *)
 Require Import BuiltIn.
 Require BuiltIn.
+Require HighOrd.
 Require bool.Bool.
 Require int.Int.
 Require map.Map.
@@ -79,7 +80,7 @@ Existing Instance stmt_WhyType.
 Axiom decide_is_skip : forall (s:stmt), (s = Sskip) \/ ~ (s = Sskip).
 
 (* Why3 assumption *)
-Definition env := (map.Map.map mident value).
+Definition env := (mident -> value).
 
 (* Why3 assumption *)
 Definition stack := (list (ident* value)%type).
@@ -116,19 +117,19 @@ Axiom eval_bin_def : forall (x:value) (op:operator) (y:value), match (x,
   end.
 
 (* Why3 assumption *)
-Fixpoint eval_term (sigma:(map.Map.map mident value)) (pi:(list (ident*
-  value)%type)) (t:term) {struct t}: value :=
+Fixpoint eval_term (sigma:(mident -> value)) (pi:(list (ident* value)%type))
+  (t:term) {struct t}: value :=
   match t with
   | (Tvalue v) => v
   | (Tvar id) => (get_stack id pi)
-  | (Tderef id) => (map.Map.get sigma id)
+  | (Tderef id) => (sigma id)
   | (Tbin t1 op t2) => (eval_bin (eval_term sigma pi t1) op (eval_term sigma
       pi t2))
   end.
 
 (* Why3 assumption *)
-Fixpoint eval_fmla (sigma:(map.Map.map mident value)) (pi:(list (ident*
-  value)%type)) (f:fmla) {struct f}: Prop :=
+Fixpoint eval_fmla (sigma:(mident -> value)) (pi:(list (ident* value)%type))
+  (f:fmla) {struct f}: Prop :=
   match f with
   | (Fterm t) => ((eval_term sigma pi t) = (Vbool true))
   | (Fand f1 f2) => (eval_fmla sigma pi f1) /\ (eval_fmla sigma pi f2)
@@ -145,70 +146,62 @@ Fixpoint eval_fmla (sigma:(map.Map.map mident value)) (pi:(list (ident*
   end.
 
 (* Why3 assumption *)
-Definition valid_fmla (p:fmla): Prop := forall (sigma:(map.Map.map mident
-  value)) (pi:(list (ident* value)%type)), (eval_fmla sigma pi p).
+Definition valid_fmla (p:fmla): Prop := forall (sigma:(mident -> value))
+  (pi:(list (ident* value)%type)), (eval_fmla sigma pi p).
 
 (* Why3 assumption *)
-Inductive one_step: (map.Map.map mident value) -> (list (ident*
-  value)%type) -> stmt -> (map.Map.map mident value) -> (list (ident*
-  value)%type) -> stmt -> Prop :=
-  | one_step_assign : forall (sigma:(map.Map.map mident value))
-      (sigma':(map.Map.map mident value)) (pi:(list (ident* value)%type))
-      (x:mident) (t:term), (sigma' = (map.Map.set sigma x (eval_term sigma pi
-      t))) -> (one_step sigma pi (Sassign x t) sigma' pi Sskip)
-  | one_step_seq_noskip : forall (sigma:(map.Map.map mident value))
-      (sigma':(map.Map.map mident value)) (pi:(list (ident* value)%type))
-      (pi':(list (ident* value)%type)) (s1:stmt) (s1':stmt) (s2:stmt),
-      (one_step sigma pi s1 sigma' pi' s1') -> (one_step sigma pi (Sseq s1
-      s2) sigma' pi' (Sseq s1' s2))
-  | one_step_seq_skip : forall (sigma:(map.Map.map mident value))
-      (pi:(list (ident* value)%type)) (s:stmt), (one_step sigma pi
-      (Sseq Sskip s) sigma pi s)
-  | one_step_if_true : forall (sigma:(map.Map.map mident value))
-      (pi:(list (ident* value)%type)) (t:term) (s1:stmt) (s2:stmt),
-      ((eval_term sigma pi t) = (Vbool true)) -> (one_step sigma pi (Sif t s1
-      s2) sigma pi s1)
-  | one_step_if_false : forall (sigma:(map.Map.map mident value))
-      (pi:(list (ident* value)%type)) (t:term) (s1:stmt) (s2:stmt),
-      ((eval_term sigma pi t) = (Vbool false)) -> (one_step sigma pi (Sif t
-      s1 s2) sigma pi s2)
-  | one_step_assert : forall (sigma:(map.Map.map mident value))
-      (pi:(list (ident* value)%type)) (f:fmla), (eval_fmla sigma pi f) ->
-      (one_step sigma pi (Sassert f) sigma pi Sskip)
-  | one_step_while_true : forall (sigma:(map.Map.map mident value))
-      (pi:(list (ident* value)%type)) (cond:term) (inv:fmla) (body:stmt),
-      ((eval_fmla sigma pi inv) /\ ((eval_term sigma pi
-      cond) = (Vbool true))) -> (one_step sigma pi (Swhile cond inv body)
-      sigma pi (Sseq body (Swhile cond inv body)))
-  | one_step_while_false : forall (sigma:(map.Map.map mident value))
-      (pi:(list (ident* value)%type)) (cond:term) (inv:fmla) (body:stmt),
-      ((eval_fmla sigma pi inv) /\ ((eval_term sigma pi
-      cond) = (Vbool false))) -> (one_step sigma pi (Swhile cond inv body)
-      sigma pi Sskip).
+Inductive one_step: (mident -> value) -> (list (ident* value)%type) ->
+  stmt -> (mident -> value) -> (list (ident* value)%type) -> stmt -> Prop :=
+  | one_step_assign : forall (sigma:(mident -> value)) (sigma':(mident ->
+      value)) (pi:(list (ident* value)%type)) (x:mident) (t:term),
+      (sigma' = (map.Map.set sigma x (eval_term sigma pi t))) -> (one_step
+      sigma pi (Sassign x t) sigma' pi Sskip)
+  | one_step_seq_noskip : forall (sigma:(mident -> value)) (sigma':(mident ->
+      value)) (pi:(list (ident* value)%type)) (pi':(list (ident*
+      value)%type)) (s1:stmt) (s1':stmt) (s2:stmt), (one_step sigma pi s1
+      sigma' pi' s1') -> (one_step sigma pi (Sseq s1 s2) sigma' pi' (Sseq s1'
+      s2))
+  | one_step_seq_skip : forall (sigma:(mident -> value)) (pi:(list (ident*
+      value)%type)) (s:stmt), (one_step sigma pi (Sseq Sskip s) sigma pi s)
+  | one_step_if_true : forall (sigma:(mident -> value)) (pi:(list (ident*
+      value)%type)) (t:term) (s1:stmt) (s2:stmt), ((eval_term sigma pi
+      t) = (Vbool true)) -> (one_step sigma pi (Sif t s1 s2) sigma pi s1)
+  | one_step_if_false : forall (sigma:(mident -> value)) (pi:(list (ident*
+      value)%type)) (t:term) (s1:stmt) (s2:stmt), ((eval_term sigma pi
+      t) = (Vbool false)) -> (one_step sigma pi (Sif t s1 s2) sigma pi s2)
+  | one_step_assert : forall (sigma:(mident -> value)) (pi:(list (ident*
+      value)%type)) (f:fmla), (eval_fmla sigma pi f) -> (one_step sigma pi
+      (Sassert f) sigma pi Sskip)
+  | one_step_while_true : forall (sigma:(mident -> value)) (pi:(list (ident*
+      value)%type)) (cond:term) (inv:fmla) (body:stmt), ((eval_fmla sigma pi
+      inv) /\ ((eval_term sigma pi cond) = (Vbool true))) -> (one_step sigma
+      pi (Swhile cond inv body) sigma pi (Sseq body (Swhile cond inv body)))
+  | one_step_while_false : forall (sigma:(mident -> value)) (pi:(list (ident*
+      value)%type)) (cond:term) (inv:fmla) (body:stmt), ((eval_fmla sigma pi
+      inv) /\ ((eval_term sigma pi cond) = (Vbool false))) -> (one_step sigma
+      pi (Swhile cond inv body) sigma pi Sskip).
 
 (* Why3 assumption *)
-Inductive many_steps: (map.Map.map mident value) -> (list (ident*
-  value)%type) -> stmt -> (map.Map.map mident value) -> (list (ident*
-  value)%type) -> stmt -> Z -> Prop :=
-  | many_steps_refl : forall (sigma:(map.Map.map mident value))
-      (pi:(list (ident* value)%type)) (s:stmt), (many_steps sigma pi s sigma
-      pi s 0%Z)
-  | many_steps_trans : forall (sigma1:(map.Map.map mident value))
-      (sigma2:(map.Map.map mident value)) (sigma3:(map.Map.map mident value))
-      (pi1:(list (ident* value)%type)) (pi2:(list (ident* value)%type))
-      (pi3:(list (ident* value)%type)) (s1:stmt) (s2:stmt) (s3:stmt) (n:Z),
-      (one_step sigma1 pi1 s1 sigma2 pi2 s2) -> ((many_steps sigma2 pi2 s2
-      sigma3 pi3 s3 n) -> (many_steps sigma1 pi1 s1 sigma3 pi3 s3
-      (n + 1%Z)%Z)).
+Inductive many_steps: (mident -> value) -> (list (ident* value)%type) ->
+  stmt -> (mident -> value) -> (list (ident* value)%type) -> stmt -> Z ->
+  Prop :=
+  | many_steps_refl : forall (sigma:(mident -> value)) (pi:(list (ident*
+      value)%type)) (s:stmt), (many_steps sigma pi s sigma pi s 0%Z)
+  | many_steps_trans : forall (sigma1:(mident -> value)) (sigma2:(mident ->
+      value)) (sigma3:(mident -> value)) (pi1:(list (ident* value)%type))
+      (pi2:(list (ident* value)%type)) (pi3:(list (ident* value)%type))
+      (s1:stmt) (s2:stmt) (s3:stmt) (n:Z), (one_step sigma1 pi1 s1 sigma2 pi2
+      s2) -> ((many_steps sigma2 pi2 s2 sigma3 pi3 s3 n) -> (many_steps
+      sigma1 pi1 s1 sigma3 pi3 s3 (n + 1%Z)%Z)).
 
-Axiom steps_non_neg : forall (sigma1:(map.Map.map mident value))
-  (sigma2:(map.Map.map mident value)) (pi1:(list (ident* value)%type))
-  (pi2:(list (ident* value)%type)) (s1:stmt) (s2:stmt) (n:Z), (many_steps
-  sigma1 pi1 s1 sigma2 pi2 s2 n) -> (0%Z <= n)%Z.
+Axiom steps_non_neg : forall (sigma1:(mident -> value)) (sigma2:(mident ->
+  value)) (pi1:(list (ident* value)%type)) (pi2:(list (ident* value)%type))
+  (s1:stmt) (s2:stmt) (n:Z), (many_steps sigma1 pi1 s1 sigma2 pi2 s2 n) ->
+  (0%Z <= n)%Z.
 
 (* Why3 assumption *)
-Definition reductible (sigma:(map.Map.map mident value)) (pi:(list (ident*
-  value)%type)) (s:stmt): Prop := exists sigma':(map.Map.map mident value),
+Definition reductible (sigma:(mident -> value)) (pi:(list (ident*
+  value)%type)) (s:stmt): Prop := exists sigma':(mident -> value),
   exists pi':(list (ident* value)%type), exists s':stmt, (one_step sigma pi s
   sigma' pi' s').
 
@@ -241,83 +234,79 @@ Axiom get_vartype_def : forall (i:ident) (pi:(list (ident* datatype)%type)),
   end.
 
 (* Why3 assumption *)
-Definition type_env := (map.Map.map mident datatype).
+Definition type_env := (mident -> datatype).
 
 (* Why3 assumption *)
-Inductive type_term: (map.Map.map mident datatype) -> (list (ident*
-  datatype)%type) -> term -> datatype -> Prop :=
-  | Type_value : forall (sigma:(map.Map.map mident datatype))
-      (pi:(list (ident* datatype)%type)) (v:value), (type_term sigma pi
-      (Tvalue v) (type_value v))
-  | Type_var : forall (sigma:(map.Map.map mident datatype)) (pi:(list (ident*
+Inductive type_term: (mident -> datatype) -> (list (ident* datatype)%type) ->
+  term -> datatype -> Prop :=
+  | Type_value : forall (sigma:(mident -> datatype)) (pi:(list (ident*
+      datatype)%type)) (v:value), (type_term sigma pi (Tvalue v)
+      (type_value v))
+  | Type_var : forall (sigma:(mident -> datatype)) (pi:(list (ident*
       datatype)%type)) (v:ident) (ty:datatype), ((get_vartype v pi) = ty) ->
       (type_term sigma pi (Tvar v) ty)
-  | Type_deref : forall (sigma:(map.Map.map mident datatype))
-      (pi:(list (ident* datatype)%type)) (v:mident) (ty:datatype),
-      ((map.Map.get sigma v) = ty) -> (type_term sigma pi (Tderef v) ty)
-  | Type_bin : forall (sigma:(map.Map.map mident datatype)) (pi:(list (ident*
+  | Type_deref : forall (sigma:(mident -> datatype)) (pi:(list (ident*
+      datatype)%type)) (v:mident) (ty:datatype), ((sigma v) = ty) ->
+      (type_term sigma pi (Tderef v) ty)
+  | Type_bin : forall (sigma:(mident -> datatype)) (pi:(list (ident*
       datatype)%type)) (t1:term) (t2:term) (op:operator) (ty1:datatype)
       (ty2:datatype) (ty:datatype), ((type_term sigma pi t1 ty1) /\
       ((type_term sigma pi t2 ty2) /\ (type_operator op ty1 ty2 ty))) ->
       (type_term sigma pi (Tbin t1 op t2) ty).
 
 (* Why3 assumption *)
-Inductive type_fmla: (map.Map.map mident datatype) -> (list (ident*
-  datatype)%type) -> fmla -> Prop :=
-  | Type_term : forall (sigma:(map.Map.map mident datatype))
-      (pi:(list (ident* datatype)%type)) (t:term), (type_term sigma pi t
-      TYbool) -> (type_fmla sigma pi (Fterm t))
-  | Type_conj : forall (sigma:(map.Map.map mident datatype))
-      (pi:(list (ident* datatype)%type)) (f1:fmla) (f2:fmla), ((type_fmla
-      sigma pi f1) /\ (type_fmla sigma pi f2)) -> (type_fmla sigma pi
-      (Fand f1 f2))
-  | Type_neg : forall (sigma:(map.Map.map mident datatype)) (pi:(list (ident*
+Inductive type_fmla: (mident -> datatype) -> (list (ident* datatype)%type) ->
+  fmla -> Prop :=
+  | Type_term : forall (sigma:(mident -> datatype)) (pi:(list (ident*
+      datatype)%type)) (t:term), (type_term sigma pi t TYbool) -> (type_fmla
+      sigma pi (Fterm t))
+  | Type_conj : forall (sigma:(mident -> datatype)) (pi:(list (ident*
+      datatype)%type)) (f1:fmla) (f2:fmla), ((type_fmla sigma pi f1) /\
+      (type_fmla sigma pi f2)) -> (type_fmla sigma pi (Fand f1 f2))
+  | Type_neg : forall (sigma:(mident -> datatype)) (pi:(list (ident*
       datatype)%type)) (f:fmla), (type_fmla sigma pi f) -> (type_fmla sigma
       pi (Fnot f))
-  | Type_implies : forall (sigma:(map.Map.map mident datatype))
-      (pi:(list (ident* datatype)%type)) (f1:fmla) (f2:fmla), (type_fmla
-      sigma pi f1) -> ((type_fmla sigma pi f2) -> (type_fmla sigma pi
-      (Fimplies f1 f2)))
-  | Type_let : forall (sigma:(map.Map.map mident datatype)) (pi:(list (ident*
+  | Type_implies : forall (sigma:(mident -> datatype)) (pi:(list (ident*
+      datatype)%type)) (f1:fmla) (f2:fmla), (type_fmla sigma pi f1) ->
+      ((type_fmla sigma pi f2) -> (type_fmla sigma pi (Fimplies f1 f2)))
+  | Type_let : forall (sigma:(mident -> datatype)) (pi:(list (ident*
       datatype)%type)) (x:ident) (t:term) (f:fmla) (ty:datatype), (type_term
       sigma pi t ty) -> ((type_fmla sigma (Init.Datatypes.cons (x, ty) pi)
       f) -> (type_fmla sigma pi (Flet x t f)))
-  | Type_forall : forall (sigma:(map.Map.map mident datatype))
-      (pi:(list (ident* datatype)%type)) (x:ident) (f:fmla) (ty:datatype),
-      (type_fmla sigma (Init.Datatypes.cons (x, ty) pi) f) -> (type_fmla
-      sigma pi (Fforall x ty f)).
+  | Type_forall : forall (sigma:(mident -> datatype)) (pi:(list (ident*
+      datatype)%type)) (x:ident) (f:fmla) (ty:datatype), (type_fmla sigma
+      (Init.Datatypes.cons (x, ty) pi) f) -> (type_fmla sigma pi (Fforall x
+      ty f)).
 
 (* Why3 assumption *)
-Inductive type_stmt: (map.Map.map mident datatype) -> (list (ident*
-  datatype)%type) -> stmt -> Prop :=
-  | Type_skip : forall (sigma:(map.Map.map mident datatype))
-      (pi:(list (ident* datatype)%type)), (type_stmt sigma pi Sskip)
-  | Type_seq : forall (sigma:(map.Map.map mident datatype)) (pi:(list (ident*
+Inductive type_stmt: (mident -> datatype) -> (list (ident* datatype)%type) ->
+  stmt -> Prop :=
+  | Type_skip : forall (sigma:(mident -> datatype)) (pi:(list (ident*
+      datatype)%type)), (type_stmt sigma pi Sskip)
+  | Type_seq : forall (sigma:(mident -> datatype)) (pi:(list (ident*
       datatype)%type)) (s1:stmt) (s2:stmt), (type_stmt sigma pi s1) ->
       ((type_stmt sigma pi s2) -> (type_stmt sigma pi (Sseq s1 s2)))
-  | Type_assigns : forall (sigma:(map.Map.map mident datatype))
-      (pi:(list (ident* datatype)%type)) (x:mident) (t:term) (ty:datatype),
-      ((map.Map.get sigma x) = ty) -> ((type_term sigma pi t ty) ->
-      (type_stmt sigma pi (Sassign x t)))
-  | Type_if : forall (sigma:(map.Map.map mident datatype)) (pi:(list (ident*
+  | Type_assigns : forall (sigma:(mident -> datatype)) (pi:(list (ident*
+      datatype)%type)) (x:mident) (t:term) (ty:datatype), ((sigma x) = ty) ->
+      ((type_term sigma pi t ty) -> (type_stmt sigma pi (Sassign x t)))
+  | Type_if : forall (sigma:(mident -> datatype)) (pi:(list (ident*
       datatype)%type)) (t:term) (s1:stmt) (s2:stmt), (type_term sigma pi t
       TYbool) -> ((type_stmt sigma pi s1) -> ((type_stmt sigma pi s2) ->
       (type_stmt sigma pi (Sif t s1 s2))))
-  | Type_assert : forall (sigma:(map.Map.map mident datatype))
-      (pi:(list (ident* datatype)%type)) (p:fmla), (type_fmla sigma pi p) ->
-      (type_stmt sigma pi (Sassert p))
-  | Type_while : forall (sigma:(map.Map.map mident datatype))
-      (pi:(list (ident* datatype)%type)) (cond:term) (body:stmt) (inv:fmla),
-      (type_fmla sigma pi inv) -> ((type_term sigma pi cond TYbool) ->
-      ((type_stmt sigma pi body) -> (type_stmt sigma pi (Swhile cond inv
-      body)))).
+  | Type_assert : forall (sigma:(mident -> datatype)) (pi:(list (ident*
+      datatype)%type)) (p:fmla), (type_fmla sigma pi p) -> (type_stmt sigma
+      pi (Sassert p))
+  | Type_while : forall (sigma:(mident -> datatype)) (pi:(list (ident*
+      datatype)%type)) (cond:term) (body:stmt) (inv:fmla), (type_fmla sigma
+      pi inv) -> ((type_term sigma pi cond TYbool) -> ((type_stmt sigma pi
+      body) -> (type_stmt sigma pi (Swhile cond inv body)))).
 
 (* Why3 assumption *)
-Definition compatible_env (sigma:(map.Map.map mident value))
-  (sigmat:(map.Map.map mident datatype)) (pi:(list (ident* value)%type))
-  (pit:(list (ident* datatype)%type)): Prop := (forall (id:mident),
-  ((type_value (map.Map.get sigma id)) = (map.Map.get sigmat id))) /\
-  forall (id:ident), ((type_value (get_stack id pi)) = (get_vartype id pit)).
+Definition compatible_env (sigma:(mident -> value)) (sigmat:(mident ->
+  datatype)) (pi:(list (ident* value)%type)) (pit:(list (ident*
+  datatype)%type)): Prop := (forall (id:mident), ((type_value (sigma
+  id)) = (sigmat id))) /\ forall (id:ident), ((type_value (get_stack id
+  pi)) = (get_vartype id pit)).
 
 Axiom type_inversion : forall (v:value),
   match (type_value v) with
@@ -326,32 +315,39 @@ Axiom type_inversion : forall (v:value),
   | TYunit => (v = Vvoid)
   end.
 
-Require Import Why3.
-
-Ltac ae := why3 "Alt-Ergo,0.99.1," timelimit 3; admit.
 
 (* Why3 goal *)
 Theorem eval_type_term : forall (t:term), forall (x:term) (x1:operator)
-  (x2:term), (t = (Tbin x x1 x2)) -> ((forall (sigma:(map.Map.map mident
-  value)) (pi:(list (ident* value)%type)) (sigmat:(map.Map.map mident
-  datatype)) (pit:(list (ident* datatype)%type)) (ty:datatype),
-  (compatible_env sigma sigmat pi pit) -> ((type_term sigmat pit x2 ty) ->
-  ((type_value (eval_term sigma pi x2)) = ty))) ->
-  ((forall (sigma:(map.Map.map mident value)) (pi:(list (ident* value)%type))
-  (sigmat:(map.Map.map mident datatype)) (pit:(list (ident* datatype)%type))
-  (ty:datatype), (compatible_env sigma sigmat pi pit) -> ((type_term sigmat
-  pit x ty) -> ((type_value (eval_term sigma pi x)) = ty))) ->
-  forall (sigma:(map.Map.map mident value)) (pi:(list (ident* value)%type))
-  (sigmat:(map.Map.map mident datatype)) (pit:(list (ident* datatype)%type))
-  (ty:datatype), (compatible_env sigma sigmat pi pit) -> ((type_term sigmat
-  pit t ty) -> ((type_value (eval_term sigma pi t)) = ty)))).
+  (x2:term), (t = (Tbin x x1 x2)) -> ((forall (sigma:(mident -> value))
+  (pi:(list (ident* value)%type)) (sigmat:(mident -> datatype))
+  (pit:(list (ident* datatype)%type)) (ty:datatype), (compatible_env sigma
+  sigmat pi pit) -> ((type_term sigmat pit x2 ty) ->
+  ((type_value (eval_term sigma pi x2)) = ty))) -> ((forall (sigma:(mident ->
+  value)) (pi:(list (ident* value)%type)) (sigmat:(mident -> datatype))
+  (pit:(list (ident* datatype)%type)) (ty:datatype), (compatible_env sigma
+  sigmat pi pit) -> ((type_term sigmat pit x ty) ->
+  ((type_value (eval_term sigma pi x)) = ty))) -> forall (sigma:(mident ->
+  value)) (pi:(list (ident* value)%type)) (sigmat:(mident -> datatype))
+  (pit:(list (ident* datatype)%type)) (ty:datatype), (compatible_env sigma
+  sigmat pi pit) -> ((type_term sigmat pit t ty) ->
+  ((type_value (eval_term sigma pi t)) = ty)))).
 (* Why3 intros t x x1 x2 h1 h2 h3 sigma pi sigmat pit ty h4 h5. *)
 intros t x x1 x2 H;rewrite H in *;clear H.
 simpl; intros.
 inversion H2; subst; clear H2.
 destruct H9 as (h1 & h2 & h3).
 generalize (type_inversion (eval_term sigma pi x)).
+rewrite (H0 sigma pi sigmat pit ty1 H1 h1).
 generalize (type_inversion (eval_term sigma pi x2)).
-destruct h3; ae.
-Admitted.
+rewrite (H sigma pi sigmat pit ty2 H1 h2).
+destruct h3; intros (n2 & hh2) (n1 & hh1); rewrite hh1 ; rewrite hh2.
+now rewrite (eval_bin_def (Vint n1) Oplus (Vint n2)).
+now rewrite (eval_bin_def (Vint n1) Ominus (Vint n2)).
+now rewrite (eval_bin_def (Vint n1) Omult (Vint n2)).
+generalize (eval_bin_def (Vint n1) Ole (Vint n2)).
+intros (ha,hb).
+destruct (Z_le_dec n1 n2) as [ l | l].
+now rewrite (ha l).
+now rewrite (hb l).
+Qed.
 
